\documentclass[a4paper]{article}
\usepackage[utf8]{inputenc}


%=-=-=-=-=-=-=-=-=-=-=-=-=-=-=-=-=-=-=-=-=-=-=-=-=-=-=-=-=-=-=-=-=-=-=-=-=-=-=-=-
% PREAMBLE
%=-=-=-=-=-=-=-=-=-=-=-=-=-=-=-=-=-=-=-=-=-=-=-=-=-=-=-=-=-=-=-=-=-=-=-=-=-=-=-=-

%%%%%%%%%%%%%%%%%%%%%%%%%%%%%%%%%%%%%%%%%%%%%%%%%%%%%%%%%%%%%%%%%%%%%
% Important styling notes
%%
% For now, to include img.jpg in img/path/to/img.jpg, just use:
% path/to/img.jpg - for details see style.tex
\input{style.tex}




\begin{document}
%=-=-=-=-=-=-=-=-=-=-=-=-=-=-=-=-=-=-=-=-=-=-=-=-=-=-=-=-=-=-=-=-=-=-=-=-=-=-=-=-
% GLOBAL STYLES (DOCUMENT SCOPE)
%=-=-=-=-=-=-=-=-=-=-=-=-=-=-=-=-=-=-=-=-=-=-=-=-=-=-=-=-=-=-=-=-=-=-=-=-=-=-=-=-
% caption: Figure 1 -> <bold> Fig. 1 </bold>
\captionsetup[figure]{labelfont={bf},labelformat={default},labelsep=period,name={Fig.}}


%=-=-=-=-=-=-=-=-=-=-=-=-=-=-=-=-=-=-=-=-=-=-=-=-=-=-=-=-=-=-=-=-=-=-=-=-=-=-=-=-
% TITLE PAGE
%=-=-=-=-=-=-=-=-=-=-=-=-=-=-=-=-=-=-=-=-=-=-=-=-=-=-=-=-=-=-=-=-=-=-=-=-=-=-=-=-
%\input{title.tex}
%\maketitle



%=-=-=-=-=-=-=-=-=-=-=-=-=-=-=-=-=-=-=-=-=-=-=-=-=-=-=-=-=-=-=-=-=-=-=-=-=-=-=-=-
% MAIN DOCUMENT
%=-=-=-=-=-=-=-=-=-=-=-=-=-=-=-=-=-=-=-=-=-=-=-=-=-=-=-=-=-=-=-=-=-=-=-=-=-=-=-=-




%------------------------------ New section ------------------------------%
\boxsimple{

Let 
\[
\bM = \begin{bmatrix}
1 & 0 & 1\\
1 & 1 & 0\\
0 & 1 & 1
\end{bmatrix}
\]
Find $\bM^{25}$  (\href{https://www.youtube.com/watch?v=7k2HmZJ_dYE}{source}).
}
\textbf{Solution:}

My solution is slightly different than the one in the video in the sense that it uses elementary matrix operations.

Matrix $\bM$ can be written as the sum of the unit matrix $\bI_3$ and another ``complement'' matrix $\bC$:
\begin{equation*}
    \bM = \bI_3 + \bC, \quad \bC = 
    \begin{bmatrix}
        0 & 0 & 1\\
        1 & 0 & 0\\
        0 & 1 & 0
    \end{bmatrix}
\end{equation*}

First, to expand $(\bI_3 + \bC)^{25}$, we use the binomial theorem (see \ref{app:binomial}):
\[
    (\bI + \bC)^{25} = \sum_{k=0}^{25}\frac{25!}{k!(25-k)!}\bI^{25-k}\bC^k = \sum_{k=0}^{25}\frac{25!}{k!(25-k)!}\bC^k
    \label{eq:sum_wrt_c}
    \tag{1}
\]
Now $\bC^k$ needs to be computed for each $k$. $\bC$ resembles with the $\bI_3$ unit matrix; we can transform $\bI_3$ to $\bC$ if we swap rows 1, 3 (operation $R_1 \leftrightarrow R_3$) and then swap rows 2, 3 (operation $R_2 \leftrightarrow R_3$):
\[
   \begin{bmatrix}
        1 & 0 & 0\\
        0 & 1 & 0\\
        0 & 0 & 1
    \end{bmatrix}
    \xrightarrow[]{R_1 \leftrightarrow R_3}
    \begin{bmatrix}
        0 & 0 & 1\\
        0 & 1 & 0\\
        1 & 0 & 0
    \end{bmatrix}
    \xrightarrow[]{R_2 \leftrightarrow R_3}
    \begin{bmatrix}
        0 & 0 & 1\\
        1 & 0 & 0\\
        0 & 1 & 0
    \end{bmatrix}
\]
Operation $R_{13}$ can be performed by matrix multiplication; by multiplying $\bI_3$ with a $3\times 3$ so called ``elementary'' matrix $\textbf{E}_{13}$ such that it swaps rows 1 and 3. So does $R_{23}$, but with $\textbf{E}_{23}$. Therefore, $\bC$ can be expressed with matrix multiplication as
\[
\bC = \textbf{E}_{23}\textbf{E}_{13} \bI_3 = \textbf{E}_{23}\textbf{E}_{13} 
\label{eq:mat_c}
\tag{2}
\]
One can find out (see \ref{app:elem_row}) that the sought row-swapping matrices $\textbf{E}_{23}$, $\textbf{E}_{13}$ are:
\[
    \textbf{E}_{23} = 
    \begin{bmatrix}
        1 & 0 & 0 \\
        0 & 0 & 1 \\
        0 & 1 & 0
    \end{bmatrix}, \quad
    \textbf{E}_{13} = 
    \begin{bmatrix}
        0 & 0 & 1 \\
        0 & 1 & 0 \\
        1 & 0 & 0
    \end{bmatrix}
\]
Computing the next higher power:
\begin{align*}
\bC^2 &= \textbf{E}_{23}\textbf{E}_{13}\bC =   \textbf{E}_{23}\textbf{E}_{13}\begin{bmatrix} 
        0 & 0 & 1\\
        1 & 0 & 0\\
        0 & 1 & 0
    \end{bmatrix} 
= \textbf{E}_{23}
    \begin{bmatrix}
        0 & 1 & 0\\
        1 & 0 & 0\\
         0 & 0 & 1\\
    \end{bmatrix}\\
&= 
    \begin{bmatrix}
        0 & 1 & 0\\
        0 & 0 & 1\\
        1 & 0 & 0\\
    \end{bmatrix}
    \label{eq:mat_c_squared}
    \tag{3}
\end{align*}
Raising to the next higher power, we obtain a nice recursion:
\begin{align*}
    \bC^3 &= \bC\bC^2\\
    &= \textbf{E}_{23}\textbf{E}_{13}\bC^2 = \textbf{E}_{23}\textbf{E}_{13} \begin{bmatrix}
            0 & 1 & 0\\
            0 & 0 & 1\\
            1 & 0 & 0\\
        \end{bmatrix}\\
    &=\textbf{E}_{23} \begin{bmatrix}
            1 & 0 & 0\\
            0 & 0 & 1\\
            0 & 1 & 0\\
        \end{bmatrix}
    = \begin{bmatrix}
            1 & 0 & 0\\
            0 & 1 & 0\\
            0 & 0 & 1\\
        \end{bmatrix} \\
    &= \bI_3
    \label{eq:mat_c_cube}
    \tag{4}
\end{align*}
In general, as derived from \eqref{eq:mat_c}, \eqref{eq:mat_c_squared}, \eqref{eq:mat_c_cube} powers of $\bC$ are repeated every 3:
\[ 
\bC^n = \left\{
\begin{array}{ll}
    \bI_3, & n = 3k, \quad k \in \setN\\
    \bC, & n = 3k+1, \quad k \in \setN\\
    \bC^2, & n = 3k+2, \quad k \in \setN\\
\end{array} 
\right. 
\]
Both $\bC$ and $\bC^2$ have been computed so the sum in \eqref{eq:sum_wrt_c} can be calculated in terms of known matrices. Notice that the term $\bC^n$ of the sum will equal to $\bI_3$ for $n=0,3,\ldots,24$, to $\bC$ for $n=1,4,\ldots,23$, and to $\bC^2$ for $n=2,5,\ldots,25$. Therefore we break the sum in 3 components, each one running for each indexing mentioned above:
\[
    \sum_{k=0}^{25}\frac{25!}{k!(25-k)!}\bC^k =
    \underbrace{\sum_{\substack{k=0, \\ k+=3}}^{24}\frac{25!}{k!(25-k)!}}_{\alpha_1}\bI_3 +
    \underbrace{\sum_{\substack{k=1, \\ k+=3}}^{23}\frac{25!}{k!(25-k)!}}_{\alpha_2}\bC +
    \underbrace{\sum_{\substack{k=2, \\ k+=3}}^{25}\frac{25!}{k!(25-k)!}}_{\alpha_3}\bC^2
\]
So we know in advance that the final will look like in terms of $\alpha_1,\; \alpha_2, \; \alpha_3$ as follows:
\[
     \sum_{k=0}^{25}\frac{25!}{k!(25-k)!}\bC^k = 
     \begin{bmatrix}
         \alpha_1 & \alpha_3 & \alpha_2\\
         \alpha_2 & \alpha_1 & \alpha_3 \\
         \alpha_3 & \alpha_2 & \alpha_1
     \end{bmatrix}
     \label{eq:sum_as_parameter_matrix}
     \tag{5}
\]
$\alpha_1,\; \alpha_2,\; \alpha_3$ can easily be computed e.g. in Python3:
\begin{verbatim}
from math import factorial as fac
a1 = sum([fac(25)/(fac(k)*fac(25-k)) for k in list(range(0,26,3))])
a2 = sum([fac(25)/(fac(k)*fac(25-k)) for k in list(range(1,26,3))])
a3 = sum([fac(25)/(fac(k)*fac(25-k)) for k in list(range(2,26,3))])
\end{verbatim}
We obtain that $\alpha_1 = \alpha_2 = 11184811$ and $\alpha_3 = 11184810$, therefore using \eqref{eq:sum_as_parameter_matrix} the final answer is
\begin{align*}
      \bM^{25} &= 
     \begin{bmatrix}
        1 & 0 & 1\\
        1 & 1 & 0\\
        0 & 1 & 1
    \end{bmatrix}^{25}  \\
     &=\sum_{k=0}^{25}\frac{25!}{k!(25-k)!}\bC^k = 
     \begin{bmatrix}
         11184811 & 11184810 & 11184811\\
         11184811 & 11184811 & 11184810 \\
         11184810 & 11184811 & 11184811
     \end{bmatrix}   
\end{align*}




%=-=-=-=-=-=-=-=-=-=-=-=-=-=-=-=-=-=-=-=-=-=-=-=-=-=-=-=-=-=-=-=-=-=-=-=-=-=-=-=-
% References
%=-=-=-=-=-=-=-=-=-=-=-=-=-=-=-=-=-=-=-=-=-=-=-=-=-=-=-=-=-=-=-=-=-=-=-=-=-=-=-=-
\newpage
\printbibliography





%=-=-=-=-=-=-=-=-=-=-=-=-=-=-=-=-=-=-=-=-=-=-=-=-=-=-=-=-=-=-=-=-=-=-=-=-=-=-=-=-
% Appendices
%=-=-=-=-=-=-=-=-=-=-=-=-=-=-=-=-=-=-=-=-=-=-=-=-=-=-=-=-=-=-=-=-=-=-=-=-=-=-=-=-
\newpage
\appendix

\section{Appendices}
% ------------------------ New appendix ------------------------ %
\newpage
\subsection{Binomial theorem}
\label{app:binomial}

\begin{theorem}[Binomial Theorem]
Let $x,y\in\setR$ and $n\geq 0$. Then
\begin{equation*}
   (x+y)^n = \sum_{k=0}^n\binom{n}{k}x^{n-k}y^k, \quad \binom{n}{k} = \frac{n!}{k!(n-k)!}
\end{equation*}
\end{theorem}

\begin{proof}
It is derived by induction as described in \cite{amsi}.
\end{proof}

% ------------------------ New appendix ------------------------ %
\newpage
\subsection{Elementary row interchange operations}
\label{app:elem_row}

We will observe and derive the elementary row interchange matrices $\textbf{E}_{ij}$, $i,j\leq 3, i \neq j$ for $3 \times 3$ matrices, however they can easily be generalised for $m \times n$. Supposed we are given a
\[
\bM = 
\begin{bmatrix}
a & b & c \\
d & e & f \\
g & h & i
\end{bmatrix}
\]
and we want to generate a new matrix $\textbf{N}$ whose 1st row is $\bM$'s 3rd row and is otherwise empty. Consider the row vectors $\be_1 = \begin{bmatrix}1 & 0 & 0\end{bmatrix}$, $\be_2 = \begin{bmatrix}0 & 1 & 0\end{bmatrix}$, $\be_3 = \begin{bmatrix}0 & 0 & 1\end{bmatrix}$. Multiplying $\be_1$ by $\textbf{M}$ extracts the 1st row of $\bM$, and so on for $\be_2$, $\be_3$:
\[
\be_1 \bM = 
\begin{bmatrix}
1 &0 &0
\end{bmatrix}
\begin{bmatrix}
a & b & c \\
d & e & f \\
g & h & i
\end{bmatrix} = 
\begin{bmatrix}
a & b & c
\end{bmatrix},
\quad \be_2 \bM = \begin{bmatrix} d & e & f \end{bmatrix}, \quad
\quad \be_3 \bM = \begin{bmatrix} g & h & i \end{bmatrix}, \quad
\]
Therefore if we multiply $\textbf{E}_{13} := \begin{bmatrix}
\be_3 & \be_2 & \be_2
\end{bmatrix}\t$ with $\bM$, the result will consist of $\bM$'s 3rd row  stacked on top of its 2nd row, stacked on top of the 1st row, i.e. $\bM$ with its rows 1 and 3 swapped:
\[
\textbf{E}_{13}\bM = 
\begin{bmatrix}
\textbf{e}_3 \\ \textbf{e}_2 \\ \textbf{e}_1
\end{bmatrix} \bM = 
\begin{bmatrix}
0 & 0 & 1\\
0 & 1 & 0 \\
1 & 0 & 0
\end{bmatrix}\bM = 
\begin{bmatrix}
g & h & i\\
d & e & f \\
a & b & c 
\end{bmatrix}
\]
Similarly, $\textbf{E}_{23}\bM$ swaps rows 2 and 3 of matrix $\bM$ and $\textbf{E}_{23}\textbf{E}_{13}\bM$ swaps row 1 with 3, and then rows 2 with 3:
\begin{gather*}
\textbf{E}_{23}\textbf{E}_{13}\bM = 
\textbf{E}_{23}
\begin{bmatrix}
g & h & i\\
d & e & f \\
a & b & c 
\end{bmatrix} = 
\begin{bmatrix}
g & h & i\\
a & b & c \\
d & e & f 
\end{bmatrix}
\end{gather*}

There's a neat property to note about the row interchange matrix $\textbf{E}_{ij}$; its inverse is itself. That should be intuitively obvious, as multiplying .e.g $\textbf{E}_{13}$ by $\bM$ swaps rows 1, 3 and multiplying again by $\textbf{E}_{13}$ swaps again rows 1,3, leading back to the original matrix $\bM$.
\begin{lemma}[inverse of row interchange matrix]
Let  $\textbf{E}_{ij}$ be an elementary row interchange matrix that swaps rows $i, j, i,j \geq m$ of an invertible matrix $\bM\in \setR^{m\times n}$. Then:
\begin{equation}
    \textbf{E}_{ij} = \textbf{E}_{ij}^{-1}
\end{equation}
\end{lemma}
\begin{proof}
\begin{gather*}
    \textbf{E}_{ij}\textbf{E}_{ij}\bM = \bM \Rightarrow \\
    \textbf{E}_{ij}\textbf{E}_{ij} = \bI_m
    \label{eq:elem_matrix_inv}
\end{gather*}
\end{proof}
Some other properties that can be readily derived from \eqref{eq:elem_matrix_inv} are:
% https://en.wikipedia.org/wiki/Exchange_matrix transpose and powers
\begin{lemma}[properties of row interchange matrices]
If $\textbf{E}_{ij}$ is an elementary matrix that interchanges rows $i$ and $j$, then:
\begin{equation}
    \textbf{E}_{ij}^n =
    \left\{
    \begin{array}{ll}
    \textbf{E}_{ij}, & n = 2k, \quad k \in \setN\\
    \bI , & n = 2k+1, \quad k \in \setN
\end{array} 
\right.
\end{equation}
Furthermore, $\textbf{E}_{ij}$ is symmetric:
\begin{equation}
    \textbf{E}_{ij}\t = \textbf{E}_{ij}
\end{equation}
\end{lemma}

\end{document}